theories/cgraph.v
@@ -77,7 +77,7 @@ Section cgraph.
 
   Lemma out_edges_in_labels g v1 v2 l :
     out_edges g v1 !! v2 = Some l ->
-    ∃ x, in_labels g v2 = {[ l ]} ⋅ x.
+    ∃ x, in_labels g v2 ≡ {[ l ]} ⋅ x.
   Proof.
   Admitted.
 
