theories/todo.md
@@ -1,8 +1,12 @@
-* think about different way to do generic invariant and separation logic
-* prove connectivity graph lemmas
-* using those prove the generic invariant lemmas
-* prove preservation using generic invariant library
-* figure out adequacy statement for generic invariant
-* prove progress using that adequacy statement
+* (? of ?) prove connectivity graph lemmas
+* (1 of 3) think about different way to do generic invariant and separation logic
+* (1 of 3) using those prove the generic invariant lemmas
+* (0.8 of 5) prove preservation using generic invariant library
+* (0 of ∞) figure out adequacy statement for generic invariant
+* (0 of ∞) prove progress using that adequacy statement
 * extensions
+  - rec lambdas
+  - recursive sessions
+  - async subtyping
+  - locks
 * write paper
